messageInvariantPrototypes/twoPhaseCommit/hosts.dfy
@@ -22,6 +22,31 @@ module CoordinatorHost {
     }
   }
 
+  ghost predicate GroupWFConstants(grp_c: seq<Constants>, participantCount: nat)
+  {
+    // There must be exactly one coordinator
+    && |grp_c| == 1
+    // The coordinator's constants must correctly account for the number of participants
+    && ConstantsValidForGroup(grp_c[0], participantCount)
+  }
+
+  ghost predicate GroupWF(grp_c: seq<Constants>, grp_v: seq<Variables>, participantCount: nat)
+  {
+    && GroupWFConstants(grp_c, participantCount)
+    // Variables size matches group size defined by grp_c
+    && |grp_v| == |grp_c|
+    // Each host is well-formed
+    && (forall hostid:HostId | hostid < |grp_c| :: grp_v[hostid].WF(grp_c[hostid]))
+  }
+
+  ghost predicate GroupInit(grp_c: seq<Constants>, grp_v: seq<Variables>)
+  {
+    // Coordinator is initialized to know about the N-1 participants.
+    && |grp_c| == 1
+    && |grp_v| == |grp_c|
+    && Init(grp_c[0], grp_v[0])
+  }
+
   ghost predicate Init(c: Constants, v: Variables)
   {
     && v.WF(c)
@@ -130,6 +155,36 @@ module ParticipantHost {
     }
   }
 
+  ghost predicate GroupWFConstants(grp_c: seq<Constants>)
+  {
+    // There must at least be a participant
+    && 0 < |grp_c|
+    // The participants's constants must match their group positions.
+    // (Actually, they just need to be distinct from one another so we get
+    // non-conflicting votes, but this is an easy way to express that property.)
+    && (forall hostid:HostId | hostid < |grp_c|
+        :: ConstantsValidForGroup(grp_c[hostid], hostid))
+  }
+
+  ghost predicate GroupWF(grp_c: seq<Constants>, grp_v: seq<Variables>)
+  {
+    && GroupWFConstants(grp_c)
+    // Variables size matches group size defined by grp_c
+    && |grp_v| == |grp_c|
+    // Each host is well-formed
+    && (forall hostid:HostId | hostid < |grp_c| :: grp_v[hostid].WF(grp_c[hostid]))
+  }
+
+  ghost predicate GroupInit(grp_c: seq<Constants>, grp_v: seq<Variables>)
+  {
+    // constants & variables are well-formed (same number of host slots as constants expect)
+    && GroupWF(grp_c, grp_v)
+    // Participants initted with their ids.
+    && (forall hostid:HostId | hostid < |grp_c| ::
+        Init(grp_c[hostid], grp_v[hostid])
+      )
+  }
+
   ghost predicate Init(c: Constants, v: Variables)
   {
     && v.sendVote == false
@@ -200,80 +255,3 @@ module ParticipantHost {
     exists step :: NextStep(c, v, v', step, msgOps)
   }
 } // end module ParticipantHost
-
-
-
-module Host {
-  import opened UtilitiesLibrary
-  import opened Types
-  import CoordinatorHost
-  import ParticipantHost
-
-  datatype Constants =
-    | CoordinatorConstants(coordinator: CoordinatorHost.Constants)
-    | ParticipantConstants(participant: ParticipantHost.Constants)
-
-  datatype Variables =
-    | CoordinatorVariables(coordinator: CoordinatorHost.Variables)
-    | ParticipantVariables(participant: ParticipantHost.Variables)
-  {
-    ghost predicate WF(c: Constants) {
-      && (CoordinatorVariables? <==> c.CoordinatorConstants?) // types of c & v agree
-      && (match c
-            case CoordinatorConstants(_) => coordinator.WF(c.coordinator)
-            case ParticipantConstants(_) => participant.WF(c.participant)
-          )
-    }
-  }
-
-
-
-  ghost predicate GroupWFConstants(grp_c: seq<Constants>)
-  {
-    // There must at least be a coordinator
-    && 0 < |grp_c|
-    // Last host is a coordinator
-    && Last(grp_c).CoordinatorConstants?
-    // All the others are participants
-    && (forall hostid:HostId | hostid < |grp_c|-1 :: grp_c[hostid].ParticipantConstants?)
-    // The coordinator's constants must correctly account for the number of participants
-    && CoordinatorHost.ConstantsValidForGroup(Last(grp_c).coordinator, |grp_c|-1)
-    // The participants's constants must match their group positions.
-    // (Actually, they just need to be distinct from one another so we get
-    // non-conflicting votes, but this is an easy way to express that property.)
-    && (forall hostid:HostId | hostid < |grp_c|-1
-        :: ParticipantHost.ConstantsValidForGroup(grp_c[hostid].participant, hostid))
-  }
-
-  ghost predicate GroupWF(grp_c: seq<Constants>, grp_v: seq<Variables>)
-  {
-    && GroupWFConstants(grp_c)
-    // Variables size matches group size defined by grp_c
-    && |grp_v| == |grp_c|
-    // Each host is well-formed
-    && (forall hostid:HostId | hostid < |grp_c| :: grp_v[hostid].WF(grp_c[hostid]))
-  }
-
-  ghost predicate GroupInit(grp_c: seq<Constants>, grp_v: seq<Variables>)
-  {
-    // constants & variables are well-formed (same number of host slots as constants expect)
-    && GroupWF(grp_c, grp_v)
-    // Coordinator is initialized to know about the N-1 participants.
-    && CoordinatorHost.Init(Last(grp_c).coordinator, Last(grp_v).coordinator)
-    // Participants initted with their ids.
-    && (forall hostid:HostId | hostid < |grp_c|-1 ::
-        ParticipantHost.Init(grp_c[hostid].participant, grp_v[hostid].participant)
-      )
-  }
-
-  // Dispatch Next to appropriate underlying implementation.
-  ghost predicate Next(c: Constants, v: Variables, v': Variables, msgOps: MessageOps)
-  {
-    && v.WF(c)
-    && v'.WF(c)
-    && (match c
-      case CoordinatorConstants(_) => CoordinatorHost.Next(c.coordinator, v.coordinator, v'.coordinator, msgOps)
-      case ParticipantConstants(_) => ParticipantHost.Next(c.participant, v.participant, v'.participant, msgOps)
-      )
-  }
-} // end module Host
